src/Utils.v
@@ -241,6 +241,20 @@ Section ListUpdate.
   Qed.
 End ListUpdate.
 
+Lemma nth_error_Some' :
+  forall [A: Type] (l: list A) (n: nat) (a: A),
+    nth_error l n = Some a ->
+    n < length l.
+Proof.
+  intros. eapply nth_error_Some. by eapply Some_not_None.
+Qed.
+Ltac saturate_list:=
+  repeat match goal with
+  | H: nth_error ?xs ?idx = Some _ |- _ =>
+      learn_hyp (nth_error_Some' _ _ _ H)
+  end.                 
+
+
 Fixpoint listSumToInl [A B: Type] (l: list (A+B)) : list A :=
   match l with
   | nil => nil
@@ -259,3 +273,10 @@ Proof.
     apply IHn.
     lia.
 Qed.
+
+Ltac simplify_nat :=
+  repeat match goal with
+  | H: _ <? _ = true |- _ => rewrite PeanoNat.Nat.ltb_lt in H
+  | H: _ <? _ = false |- _ => rewrite PeanoNat.Nat.ltb_nlt in H
+  | _ => lia                                                                       
+  end.
